<?xml version="1.0"?>
<rdf:RDF
    xmlns:rdf="http://www.w3.org/1999/02/22-rdf-syntax-ns#"
    xmlns:dc="http://purl.org/dc/terms/"
    xmlns:j.0="http://purl.org/dc/elements/1.1/"
    xmlns:schema="https://schema.org/"
    xmlns:dano="https://w3id.org/dano#"
    xmlns:owl="http://www.w3.org/2002/07/owl#"
    xmlns:skos="http://www.w3.org/2004/02/skos/core#"
    xmlns:geo="http://www.opengis.net/ont/geosparql#"
    xmlns:rdfs="http://www.w3.org/2000/01/rdf-schema#"
    xmlns:vann="http://purl.org/vocab/vann/"
    xmlns:foaf="http://xmlns.com/foaf/0.1/"
    xmlns:xsd="http://www.w3.org/2001/XMLSchema#"
  xml:base="https://w3id.org/dano" > 
  <rdf:Description rdf:about="http://purl.org/dc/elements/1.1/format">
    <rdfs:label xml:lang="en">Format</rdfs:label>
    <rdfs:isDefinedBy rdf:resource="http://purl.org/dc/elements/1.1/"/>
    <rdfs:comment xml:lang="en">The file format, physical medium, or dimensions of the resource.</rdfs:comment>
  </rdf:Description>
  <rdf:Description rdf:nodeID="A0">
    <rdf:type rdf:resource="http://www.w3.org/2002/07/owl#Restriction"/>
    <owl:minQualifiedCardinality rdf:datatype="http://www.w3.org/2001/XMLSchema#nonNegativeInteger">2</owl:minQualifiedCardinality>
    <owl:onProperty rdf:resource="#contains"/>
    <owl:onClass rdf:resource="#TextElement"/>
  </rdf:Description>
  <rdf:Description rdf:about="http://purl.org/dc/elements/1.1/identifier">
    <rdfs:label xml:lang="en">Identifier</rdfs:label>
    <rdfs:isDefinedBy rdf:resource="http://purl.org/dc/elements/1.1/"/>
    <rdfs:comment xml:lang="en">An unambiguous reference to the resource within a given context.</rdfs:comment>
  </rdf:Description>
  <rdf:Description rdf:about="https://schema.org/domainIncludes">
    <rdf:type rdf:resource="http://www.w3.org/2002/07/owl#AnnotationProperty"/>
  </rdf:Description>
  <rdf:Description rdf:about="http://purl.org/dc/elements/1.1/source">
    <rdfs:label xml:lang="en">Source</rdfs:label>
    <rdfs:isDefinedBy rdf:resource="http://purl.org/dc/elements/1.1/"/>
    <rdfs:comment xml:lang="en">A related resource from which the described resource is derived.</rdfs:comment>
  </rdf:Description>
  <rdf:Description rdf:about="#Dimension_1">
    <rdfs:label>Dimension</rdfs:label>
    <rdf:type rdf:resource="#Dimension"/>
  </rdf:Description>
  <rdf:Description rdf:about="http://purl.org/dc/elements/1.1/title">
    <rdfs:label xml:lang="en">Title</rdfs:label>
    <rdfs:isDefinedBy rdf:resource="http://purl.org/dc/elements/1.1/"/>
    <rdfs:comment xml:lang="en">A name given to the resource.</rdfs:comment>
  </rdf:Description>
  <rdf:Description rdf:about="#hasMeta">
    <rdfs:range rdf:resource="#DrawingElementMeta"/>
    <rdfs:label>has meta</rdfs:label>
    <rdfs:domain rdf:resource="#DrawingElement"/>
    <rdfs:comment>Links meta information to a drawing element.</rdfs:comment>
    <rdf:type rdf:resource="http://www.w3.org/2002/07/owl#ObjectProperty"/>
  </rdf:Description>
  <rdf:Description rdf:about="#hasGeometry">
    <rdfs:label>has geometry</rdfs:label>
    <rdfs:domain rdf:resource="#DrawingElement"/>
    <rdfs:comment>Links the drawing element to its geometrical representation.</rdfs:comment>
    <rdf:type rdf:resource="http://www.w3.org/2002/07/owl#ObjectProperty"/>
  </rdf:Description>
  <rdf:Description rdf:about="http://www.opengis.net/ont/geosparql#hasGeometry">
    <rdfs:label xml:lang="en">hasGeometry</rdfs:label>
    <rdfs:isDefinedBy rdf:resource="http://www.opengis.net/spec/geosparql/1.0"/>
    <rdfs:isDefinedBy rdf:resource="http://www.opengis.net/ont/geosparql"/>
    <rdfs:comment xml:lang="en">
      A spatial representation for a given feature.
    </rdfs:comment>
    <rdf:type rdf:resource="http://www.w3.org/2002/07/owl#ObjectProperty"/>
  </rdf:Description>
  <rdf:Description rdf:nodeID="A1">
    <owl:qualifiedCardinality rdf:datatype="http://www.w3.org/2001/XMLSchema#nonNegativeInteger">1</owl:qualifiedCardinality>
    <rdf:type rdf:resource="http://www.w3.org/2002/07/owl#Restriction"/>
    <owl:onClass rdf:resource="#TextElement"/>
    <owl:onProperty rdf:resource="#contains"/>
  </rdf:Description>
  <rdf:Description rdf:nodeID="A2">
    <rdf:type rdf:resource="http://www.w3.org/2002/07/owl#Restriction"/>
    <owl:qualifiedCardinality rdf:datatype="http://www.w3.org/2001/XMLSchema#nonNegativeInteger">2</owl:qualifiedCardinality>
    <owl:onClass rdf:resource="#Terminator"/>
    <owl:onProperty rdf:resource="#contains"/>
  </rdf:Description>
  <rdf:Description rdf:about="#isText">
    <rdfs:range rdf:resource="http://www.w3.org/2001/XMLSchema#string"/>
    <rdfs:label>is text</rdfs:label>
    <rdfs:domain rdf:resource="#TextElement"/>
    <rdfs:comment>Indicates that the description element is a text element containing the specified string.</rdfs:comment>
    <rdf:type rdf:resource="http://www.w3.org/2002/07/owl#DatatypeProperty"/>
  </rdf:Description>
  <rdf:Description rdf:about="#inferredBy">
    <rdfs:range rdf:resource="http://www.w3.org/2001/XMLSchema#string"/>
    <rdfs:label>inferred by</rdfs:label>
    <rdfs:domain rdf:resource="#DrawingElementMeta"/>
    <rdfs:comment>Indicates the actor, company, or software that inferred the drawing element.</rdfs:comment>
    <rdf:type rdf:resource="http://www.w3.org/2002/07/owl#DatatypeProperty"/>
  </rdf:Description>
  <rdf:Description rdf:about="#hasIfcRepresentation">
    <rdfs:label>has IFC representation</rdfs:label>
    <rdfs:domain rdf:resource="#DrawingElement"/>
    <rdfs:comment>Specifies the IFC representation of the drawing element.</rdfs:comment>
    <rdf:type rdf:resource="http://www.w3.org/2002/07/owl#DatatypeProperty"/>
  </rdf:Description>
  <rdf:Description rdf:about="#DisplayElement">
    <rdfs:subClassOf rdf:resource="#DrawingElement"/>
    <rdfs:label>Display Element</rdfs:label>
    <rdfs:comment>An element representing a real-world component.</rdfs:comment>
    <rdf:type rdf:resource="http://www.w3.org/2002/07/owl#Class"/>
  </rdf:Description>
  <rdf:Description rdf:about="#DescriptionElement">
    <rdfs:subClassOf rdf:resource="#DrawingElement"/>
    <rdfs:label>Description Element</rdfs:label>
    <rdfs:comment>An abstract element in a drawing describing properties of display elements. For instance, a dimension line describing a wall or a text element specifying a schematic pump symbol.</rdfs:comment>
    <rdf:type rdf:resource="http://www.w3.org/2002/07/owl#Class"/>
  </rdf:Description>
  <rdf:Description rdf:nodeID="A3">
    <schema:name>Ruhr-Universität Bochum</schema:name>
    <schema:identifier rdf:resource="https://www.inf.bi.ruhr-uni-bochum.de/iib/lehrstuhl/mitarbeiter/phillip_schoenfelder.html.en"/>
  </rdf:Description>
  <rdf:Description rdf:about="#endsWith">
    <rdfs:subPropertyOf rdf:resource="#contains"/>
    <rdfs:range rdf:resource="#Terminator"/>
    <rdfs:label>ends with</rdfs:label>
    <rdfs:domain rdf:resource="#DimensionLine"/>
    <rdfs:comment>Indicates that a dimension line ends with a dimension line marker.</rdfs:comment>
    <rdf:type rdf:resource="http://www.w3.org/2002/07/owl#ObjectProperty"/>
  </rdf:Description>
  <rdf:Description rdf:about="#DimensionChain">
    <rdfs:subClassOf rdf:nodeID="A4"/>
    <rdfs:subClassOf rdf:resource="#Composite"/>
    <rdfs:label>Dimension Chain</rdfs:label>
    <rdfs:comment>A sequence of dimensions connected together to represent cumulative measurements.</rdfs:comment>
    <rdf:type rdf:resource="http://www.w3.org/2002/07/owl#Class"/>
  </rdf:Description>
  <rdf:Description rdf:about="#refersTo">
    <owl:inverseOf rdf:resource="#isReferredToBy"/>
    <rdfs:range rdf:resource="#Terminator"/>
    <rdfs:label>refers to</rdfs:label>
    <rdfs:domain rdf:resource="#Terminator"/>
    <rdfs:comment>Indicates that the subject dimension line marker refers to another dimension line marker.</rdfs:comment>
    <rdf:type rdf:resource="http://www.w3.org/2002/07/owl#ObjectProperty"/>
  </rdf:Description>
  <rdf:Description rdf:about="http://purl.org/dc/elements/1.1/publisher">
    <rdfs:label xml:lang="en">Publisher</rdfs:label>
    <rdfs:isDefinedBy rdf:resource="http://purl.org/dc/elements/1.1/"/>
    <rdfs:comment xml:lang="en">An entity responsible for making the resource available.</rdfs:comment>
  </rdf:Description>
  <rdf:Description rdf:about="">
    <skos:historyNote>  
  v0.1: initial ontology
  
  v0.2: added cardinality constraints to the taxonomy, restructured taxonomy, modified image
 </skos:historyNote>
    <dc:modified rdf:datatype="http://www.w3.org/2001/XMLSchema#date">2025-07-15</dc:modified>
    <vann:preferredNamespaceUri rdf:resource=""/>
    <dc:publisher rdf:nodeID="A5"/>
    <dc:source rdf:resource="https://github.com/RUB-Informatik-im-Bauwesen/dano"/>
    <owl:versionIRI rdf:resource=""/>
    <dc:license rdf:resource="https://creativecommons.org/licenses/by/4.0/"/>
    <dc:creator rdf:nodeID="A6"/>
    <dc:description xml:lang="en">This ontology covers concepts of technical drawings from the perspective of computer vision-based drawing analysis to be used in collaborative settings or for post-processing. 
The preferred namespace prefix is `dano` for the namespace IRI [https://w3id.org/dano](https://w3id.org/dano).</dc:description>
    <dc:rights>Copyright 2025 by Phillip Schönfelder</dc:rights>
    <dc:issued rdf:datatype="http://www.w3.org/2001/XMLSchema#date">2025-03-11</dc:issued>
    <vann:preferredNamespacePrefix>dano</vann:preferredNamespacePrefix>
    <owl:versionInfo>v0.2</owl:versionInfo>
    <rdf:type rdf:resource="http://www.w3.org/2002/07/owl#Ontology"/>
    <dc:title xml:lang="en">Drawing Analyis Ontology (DAnO)</dc:title>
  </rdf:Description>
  <rdf:Description rdf:about="https://schema.org/rangeIncludes">
    <rdf:type rdf:resource="http://www.w3.org/2002/07/owl#AnnotationProperty"/>
  </rdf:Description>
  <rdf:Description rdf:about="#inferredFrom">
    <rdfs:range rdf:resource="http://www.w3.org/2001/XMLSchema#string"/>
    <rdfs:label>inferred from</rdfs:label>
    <rdfs:domain rdf:resource="#DrawingElementMeta"/>
    <rdfs:comment>Specifies the origin file from which the drawing element was extracted.</rdfs:comment>
    <rdf:type rdf:resource="http://www.w3.org/2002/07/owl#DatatypeProperty"/>
  </rdf:Description>
  <rdf:Description rdf:about="#AxisLine">
    <rdfs:label>Axis Line</rdfs:label>
    <rdfs:subClassOf rdf:resource="#Line"/>
    <rdf:type rdf:resource="http://www.w3.org/2002/07/owl#Class"/>
  </rdf:Description>
  <rdf:Description rdf:about="#isContainedIn">
    <owl:inverseOf rdf:resource="#contains"/>
    <rdfs:range rdf:resource="#DrawingElement"/>
    <rdfs:label>is contained in</rdfs:label>
    <rdfs:domain rdf:resource="#DrawingElement"/>
    <rdfs:comment>Indicates that the subject drawing element is part of another drawing element.</rdfs:comment>
    <rdf:type rdf:resource="http://www.w3.org/2002/07/owl#ObjectProperty"/>
  </rdf:Description>
  <rdf:Description rdf:about="#TextField">
    <rdfs:subClassOf rdf:nodeID="A0"/>
    <rdfs:subClassOf rdf:resource="#Composite"/>
    <rdfs:label>Text Field</rdfs:label>
    <rdfs:comment>A composite element containing multiple text elements, typically for multiline text.</rdfs:comment>
    <rdf:type rdf:resource="http://www.w3.org/2002/07/owl#Class"/>
  </rdf:Description>
  <rdf:Description rdf:nodeID="A4">
    <owl:onProperty rdf:resource="#contains"/>
    <owl:onClass rdf:resource="#Dimension"/>
    <rdf:type rdf:resource="http://www.w3.org/2002/07/owl#Restriction"/>
    <owl:minQualifiedCardinality rdf:datatype="http://www.w3.org/2001/XMLSchema#nonNegativeInteger">2</owl:minQualifiedCardinality>
  </rdf:Description>
  <rdf:Description rdf:about="#SectionSymbol">
    <rdfs:comment>A symbol defining the section plane that opens up a view section. Must have a partner symbol and is referred to by a TextElement which is its reference letter.</rdfs:comment>
    <rdfs:label>Section Symbol</rdfs:label>
    <rdfs:subClassOf rdf:resource="#Symbol"/>
    <rdf:type rdf:resource="http://www.w3.org/2002/07/owl#Class"/>
  </rdf:Description>
  <rdf:Description rdf:about="http://purl.org/dc/elements/1.1/relation">
    <rdfs:label xml:lang="en">Relation</rdfs:label>
    <rdfs:isDefinedBy rdf:resource="http://purl.org/dc/elements/1.1/"/>
    <rdfs:comment xml:lang="en">A related resource.</rdfs:comment>
  </rdf:Description>
  <rdf:Description rdf:about="#describes">
    <owl:inverseOf rdf:resource="#isDescribedBy"/>
    <rdfs:range rdf:resource="#DisplayElement"/>
    <rdfs:label>describes</rdfs:label>
    <rdfs:domain rdf:resource="#DescriptionElement"/>
    <rdfs:comment>Establishes the relationship between a description element and a display element, where the description element describes the display element.</rdfs:comment>
    <rdf:type rdf:resource="http://www.w3.org/2002/07/owl#ObjectProperty"/>
  </rdf:Description>
  <rdf:Description rdf:about="#inferredAt">
    <rdfs:range rdf:resource="http://www.w3.org/2001/XMLSchema#date"/>
    <rdfs:label>inferred at</rdfs:label>
    <rdfs:domain rdf:resource="#DrawingElementMeta"/>
    <rdfs:comment>Specifies the date when the drawing element was inferred.</rdfs:comment>
    <rdf:type rdf:resource="http://www.w3.org/2002/07/owl#DatatypeProperty"/>
  </rdf:Description>
  <rdf:Description rdf:about="#depicts">
    <rdfs:label>depicts</rdfs:label>
    <rdfs:domain rdf:resource="#DisplayElement"/>
    <rdfs:comment>Indicates that the subject display element graphically represents a real-world object, such as a building element, zone, or machine part.</rdfs:comment>
    <rdf:type rdf:resource="http://www.w3.org/2002/07/owl#ObjectProperty"/>
  </rdf:Description>
  <rdf:Description rdf:about="#DrawingElementMeta">
    <rdfs:subClassOf rdf:resource="http://www.w3.org/2002/07/owl#Thing"/>
    <rdfs:label>Drawing Element Meta</rdfs:label>
    <rdfs:comment>Metadata for drawing elements, including inference confidence and methods used.</rdfs:comment>
    <rdf:type rdf:resource="http://www.w3.org/2002/07/owl#Class"/>
  </rdf:Description>
  <rdf:Description rdf:about="#inferredWith">
    <rdfs:range rdf:resource="http://www.w3.org/2001/XMLSchema#string"/>
    <rdfs:label>inferred with</rdfs:label>
    <rdfs:domain rdf:resource="#DrawingElementMeta"/>
    <rdfs:comment>Indicates the algorithm used to infer the drawing element.</rdfs:comment>
    <rdf:type rdf:resource="http://www.w3.org/2002/07/owl#DatatypeProperty"/>
  </rdf:Description>
  <rdf:Description rdf:about="#contains">
    <owl:inverseOf rdf:resource="#isContainedIn"/>
    <rdfs:range rdf:resource="#DrawingElement"/>
    <rdfs:label>contains</rdfs:label>
    <rdfs:domain rdf:resource="#DrawingElement"/>
    <rdfs:comment>Indicates that the subject drawing element contains the object drawing element. For instance, lines can contain two endpoints.</rdfs:comment>
    <rdf:type rdf:resource="http://www.w3.org/2002/07/owl#TransitiveProperty"/>
    <rdf:type rdf:resource="http://www.w3.org/2002/07/owl#ObjectProperty"/>
  </rdf:Description>
  <rdf:Description rdf:about="#isDepictedBy">
    <rdfs:range rdf:resource="#DisplayElement"/>
    <rdfs:comment>Indicates that the real-world subject is depicted by the object display element, which is typically a geometric representation.</rdfs:comment>
    <rdf:type rdf:resource="http://www.w3.org/2002/07/owl#ObjectProperty"/>
    <owl:inverseOf rdf:resource="#depicts"/>
    <rdfs:label>isDepictedBy</rdfs:label>
  </rdf:Description>
  <rdf:Description rdf:about="#DrawingElement">
    <rdfs:subClassOf rdf:resource="http://www.w3.org/2002/07/owl#Thing"/>
    <rdfs:label>Drawing Element</rdfs:label>
    <rdfs:comment>A visual element in a drawing. Metadata for these elements are stored as DrawingElementMeta instances.</rdfs:comment>
    <rdf:type rdf:resource="http://www.w3.org/2002/07/owl#Class"/>
  </rdf:Description>
  <rdf:Description rdf:about="#EquipmentSymbol">
    <rdfs:label>Equipment symbol</rdfs:label>
    <rdfs:subClassOf rdf:resource="#Symbol"/>
    <rdf:type rdf:resource="http://www.w3.org/2002/07/owl#Class"/>
  </rdf:Description>
  <rdf:Description rdf:about="http://www.opengis.net/ont/geosparql">
    <owl:versionInfo>OGC GeoSPARQL 1.0</owl:versionInfo>
    <owl:versionIRI rdf:resource="http://www.opengis.net/ont/geosparql/1.0"/>
    <rdfs:seeAlso rdf:resource="http://www.opengis.net/doc/IS/geosparql/1.0"/>
    <rdfs:seeAlso rdf:resource="http://www.opengis.net/def/rule/ogc-geosparql/1.0"/>
    <rdfs:seeAlso rdf:resource="http://www.opengis.net/def/function/ogc-geosparql/1.0"/>
    <j.0:title>GeoSPARQL Ontology</j.0:title>
    <j.0:source>OGC GeoSPARQL – A Geographic Query Language for RDF Data OGC 11-052r5</j.0:source>
    <j.0:source rdf:resource="http://www.opengis.net/doc/IS/geosparql/1.0"/>
  </rdf:Description>
  <rdf:Description rdf:about="#Composite">
    <rdfs:subClassOf rdf:resource="#DescriptionElement"/>
    <rdfs:label>Composite</rdfs:label>
    <rdfs:comment>A composite element that aggregates multiple description elements.</rdfs:comment>
    <rdf:type rdf:resource="http://www.w3.org/2002/07/owl#Class"/>
  </rdf:Description>
  <rdf:Description rdf:about="http://purl.org/dc/elements/1.1/coverage">
    <rdfs:label xml:lang="en">Coverage</rdfs:label>
    <rdfs:isDefinedBy rdf:resource="http://purl.org/dc/elements/1.1/"/>
    <rdfs:comment xml:lang="en">The spatial or temporal topic of the resource, the spatial applicability of the resource, or the jurisdiction under which the resource is relevant.</rdfs:comment>
  </rdf:Description>
  <rdf:Description rdf:about="#isDescribedBy">
    <owl:inverseOf rdf:resource="#describes"/>
    <rdfs:range rdf:resource="#DescriptionElement"/>
    <rdfs:label>is described by</rdfs:label>
    <rdfs:domain rdf:resource="#DisplayElement"/>
    <rdfs:comment>Indicates that the display element is described by a description element.</rdfs:comment>
    <rdf:type rdf:resource="http://www.w3.org/2002/07/owl#ObjectProperty"/>
  </rdf:Description>
  <rdf:Description rdf:about="https://schema.org/codeRepository">
    <rdf:type rdf:resource="http://www.w3.org/2002/07/owl#Thing"/>
  </rdf:Description>
  <rdf:Description rdf:about="#Terminator">
    <rdfs:subClassOf rdf:resource="#Symbol"/>
    <rdfs:label>Terminator</rdfs:label>
    <rdfs:comment>A marker used to indicate endpoints or reference points on a dimension line.</rdfs:comment>
    <rdf:type rdf:resource="http://www.w3.org/2002/07/owl#Class"/>
  </rdf:Description>
  <rdf:Description rdf:about="#Dimension">
    <rdfs:subClassOf rdf:nodeID="A2"/>
    <rdfs:subClassOf rdf:nodeID="A7"/>
    <rdfs:subClassOf rdf:nodeID="A1"/>
    <rdfs:subClassOf rdf:resource="#Composite"/>
    <rdfs:label>Dimension</rdfs:label>
    <rdfs:comment>A composite element, comprising exactly 1 DimensionLine, 2 Terminators (at the line's ends), and 1 TextElement (for the dimension value).</rdfs:comment>
    <rdf:type rdf:resource="http://www.w3.org/2002/07/owl#Class"/>
  </rdf:Description>
  <rdf:Description rdf:about="#hasConfidence">
    <rdfs:range rdf:resource="http://www.w3.org/2001/XMLSchema#decimal"/>
    <rdfs:label>has confidence</rdfs:label>
    <rdfs:domain rdf:resource="#DrawingElement"/>
    <rdfs:comment>Specifies the confidence level of the inference that identified the drawing element.</rdfs:comment>
    <rdf:type rdf:resource="http://www.w3.org/2002/07/owl#DatatypeProperty"/>
  </rdf:Description>
  <rdf:Description rdf:nodeID="A6">
    <schema:name>Phillip Schönfelder</schema:name>
    <schema:memberOf rdf:nodeID="A3"/>
    <schema:identifier rdf:resource="https://orcid.org/0000-0002-8685-436X"/>
    <schema:email rdf:resource="mailto:phillip.schoenfelder@rub.de"/>
    <rdf:type rdf:resource="https://schema.org/Person"/>
  </rdf:Description>
  <rdf:Description rdf:about="#Line">
    <rdfs:subClassOf rdf:resource="#DescriptionElement"/>
    <rdfs:label>Line</rdfs:label>
    <rdfs:comment>A linear description element in a drawing.</rdfs:comment>
    <rdf:type rdf:resource="http://www.w3.org/2002/07/owl#Class"/>
  </rdf:Description>
  <rdf:Description rdf:about="http://purl.org/dc/elements/1.1/subject">
    <rdfs:label xml:lang="en">Subject</rdfs:label>
    <rdfs:isDefinedBy rdf:resource="http://purl.org/dc/elements/1.1/"/>
    <rdfs:comment xml:lang="en">The topic of the resource.</rdfs:comment>
  </rdf:Description>
  <rdf:Description rdf:nodeID="A5">
    <foaf:name>Chair of Computing in Engineering</foaf:name>
    <foaf:homepage rdf:resource="http://www.inf.bi.rub.de"/>
    <rdf:type rdf:resource="http://xmlns.com/foaf/0.1/Organization"/>
  </rdf:Description>
  <rdf:Description rdf:about="http://purl.org/dc/elements/1.1/type">
    <rdfs:label xml:lang="en">Type</rdfs:label>
    <rdfs:isDefinedBy rdf:resource="http://purl.org/dc/elements/1.1/"/>
    <rdfs:comment xml:lang="en">The nature or genre of the resource.</rdfs:comment>
  </rdf:Description>
  <rdf:Description rdf:about="http://purl.org/dc/elements/1.1/rights">
    <rdfs:label xml:lang="en">Rights</rdfs:label>
    <rdfs:isDefinedBy rdf:resource="http://purl.org/dc/elements/1.1/"/>
    <rdfs:comment xml:lang="en">Information about rights held in and over the resource.</rdfs:comment>
  </rdf:Description>
  <rdf:Description rdf:about="http://www.w3.org/2001/XMLSchema#date">
    <rdf:type rdf:resource="http://www.w3.org/2000/01/rdf-schema#Datatype"/>
  </rdf:Description>
  <rdf:Description rdf:about="http://purl.org/dc/elements/1.1/language">
    <rdfs:seeAlso rdf:resource="http://www.ietf.org/rfc/rfc4646.txt"/>
    <rdfs:label xml:lang="en">Language</rdfs:label>
    <rdfs:isDefinedBy rdf:resource="http://purl.org/dc/elements/1.1/"/>
    <rdfs:comment xml:lang="en">A language of the resource.</rdfs:comment>
  </rdf:Description>
  <rdf:Description rdf:nodeID="A7">
    <owl:onProperty rdf:resource="#contains"/>
    <owl:onClass rdf:resource="#DimensionLine"/>
    <rdf:type rdf:resource="http://www.w3.org/2002/07/owl#Restriction"/>
    <owl:qualifiedCardinality rdf:datatype="http://www.w3.org/2001/XMLSchema#nonNegativeInteger">1</owl:qualifiedCardinality>
  </rdf:Description>
  <rdf:Description rdf:about="#isReferredToBy">
    <owl:inverseOf rdf:resource="#refersTo"/>
    <rdfs:range rdf:resource="#Terminator"/>
    <rdfs:label>is referred to by</rdfs:label>
    <rdfs:domain rdf:resource="#Terminator"/>
    <rdfs:comment>Indicates that the subject dimension line marker is referred to by another dimension line marker.</rdfs:comment>
    <rdf:type rdf:resource="http://www.w3.org/2002/07/owl#ObjectProperty"/>
  </rdf:Description>
  <rdf:Description rdf:about="http://www.opengis.net/ont/geosparql#defaultGeometry">
    <rdfs:subPropertyOf rdf:resource="http://www.opengis.net/ont/geosparql#hasGeometry"/>
    <rdfs:label xml:lang="en">defaultGeometry</rdfs:label>
    <rdfs:isDefinedBy rdf:resource="http://www.opengis.net/spec/geosparql/1.0"/>
    <rdfs:isDefinedBy rdf:resource="http://www.opengis.net/ont/geosparql"/>
    <rdfs:comment xml:lang="en">
      The default geometry to be used in spatial calculations.
      It is Usually the most detailed geometry.
    </rdfs:comment>
    <rdf:type rdf:resource="http://www.w3.org/2002/07/owl#ObjectProperty"/>
  </rdf:Description>
  <rdf:Description rdf:about="#TextElement">
    <rdfs:subClassOf rdf:resource="#DescriptionElement"/>
    <rdfs:label>Text Element</rdfs:label>
    <rdfs:comment>A text-based description element in a drawing.</rdfs:comment>
    <rdf:type rdf:resource="http://www.w3.org/2002/07/owl#Class"/>
  </rdf:Description>
  <rdf:Description rdf:about="#Symbol">
    <rdfs:subClassOf rdf:resource="#DescriptionElement"/>
    <rdfs:label>Symbol</rdfs:label>
    <rdfs:comment>A symbolic description element representing various annotations or markers.</rdfs:comment>
    <rdf:type rdf:resource="http://www.w3.org/2002/07/owl#Class"/>
  </rdf:Description>
  <rdf:Description rdf:about="#DimensionLine">
    <rdfs:subClassOf rdf:resource="#Line"/>
    <rdfs:label>Dimension Line</rdfs:label>
    <rdfs:comment>The line type for indicating dimensions in a drawing, typically used to represent measurements.</rdfs:comment>
    <rdf:type rdf:resource="http://www.w3.org/2002/07/owl#Class"/>
  </rdf:Description>
</rdf:RDF>

<!-- Created with TopBraid -->
